{
 "metadata": {
  "language_info": {
   "name": "python",
   "version": "3.8.10",
   "mimetype": "text/x-python",
   "codemirror_mode": {
    "name": "ipython",
    "version": 3
   },
   "pygments_lexer": "ipython3",
   "nbconvert_exporter": "python",
   "file_extension": ".py"
  },
  "orig_nbformat": 4,
  "kernelspec": {
   "name": "python3",
   "display_name": "Python 3.8.10 64-bit ('penter': conda)"
  },
  "interpreter": {
   "hash": "66a9b9246fc3be4ca617a120a8795ea86c1f91adc8c4462264e6f2ff62103632"
  }
 },
 "nbformat": 4,
 "nbformat_minor": 2,
 "cells": [
  {
   "cell_type": "code",
   "execution_count": 1,
   "source": [
    "%matplotlib inline\r\n",
    "import numpy as np\r\n",
    "import matplotlib.pyplot as plt\r\n",
    "from matplotlib.patches import Polygon\r\n",
    "from matplotlib.collections import PatchCollection\r\n",
    "import seaborn as sns\r\n",
    "plt.rcParams['text.usetex'] = True"
   ],
   "outputs": [],
   "metadata": {}
  },
  {
   "cell_type": "markdown",
   "source": [
    "# The Matrix Cookbook\r\n",
    "[原文](https://www.math.uwaterloo.ca/~hwolkowi/matrixcookbook.pdf)\r\n",
    "## 符号和命名\r\n",
    "$\\mathbf{A}\\rightarrow\\;$ Matrix\r\n",
    "\r\n",
    "$\\mathbf{A}_{ij}\\rightarrow\\;$ Matrix indexed for some purpose\r\n",
    "\r\n",
    "$\\mathbf{A}_{i}\\rightarrow\\;$ Matrix indexed for some purpose\r\n",
    "\r\n",
    "$\\mathbf{A}^{ij}\\rightarrow\\;$ Matrix indexed for some purpose\r\n",
    "\r\n",
    "$\\mathbf{A}^{n}\\rightarrow\\;$ Matrix indexed for some purpose or the the $n^{th}$ power of a square matrix\r\n",
    "\r\n",
    "$\\mathbf{A}^{-1}\\rightarrow\\;$ The inverse matrix of matrix $\\mathbf{A}$\r\n",
    "\r\n",
    "$\\mathbf{A}^{\\dagger}\\rightarrow\\;$ The pseudo inverse matrix of the matrix $\\mathbf{A}$\r\n",
    "\r\n",
    "$\\mathbf{A}^{1/2}\\rightarrow\\;$ The square root of a matrix (if unique), not elementwise\r\n",
    "\r\n",
    "$(\\mathbf{A})_{i,j}\\rightarrow\\;$ The $(i,j)^{th}$ entry of the matrix $\\mathbf{A}$\r\n",
    "\r\n",
    "$\\mathbf{A}_{i,j}\\rightarrow\\;$ The $(i,j)^{th}$ entry of the matrix $\\mathbf{A}$\r\n",
    "\r\n",
    "$[\\mathbf{A}]_{i,j}\\rightarrow\\;$ The $ij$-suubmatrix, i.e. $\\mathbf{A}$ with $i^{th}$ row and $j^{th}$ column deleted\r\n",
    "\r\n",
    "$\\vec{a}\\rightarrow\\;$ Vector (column-vector)\r\n",
    "\r\n",
    "$\\vec{a}_{i}\\rightarrow\\;$ Vector indexed for some purpose\r\n",
    "\r\n",
    "$\\alpha_{i}\\rightarrow\\;$ The $i^{th}$ element of vector $\\vec{a}$\r\n",
    "\r\n",
    "$\\alpha\\rightarrow\\;$ Scalar\r\n",
    "\r\n",
    "---\r\n",
    "\r\n",
    "$\\Re z\\rightarrow\\;$ Real part of a scalar\r\n",
    "\r\n",
    "$\\Re \\mathbf{z}\\rightarrow\\;$ Real part of a vectorS\r\n",
    "\r\n",
    "$\\Re \\mathbf{Z}\\rightarrow\\;$ Real part of a matrix\r\n",
    "\r\n",
    "$\\Im z\\rightarrow\\;$ Imaginary part of a scalar\r\n",
    "\r\n",
    "$\\Im \\mathbf{z}\\rightarrow\\;$ Imaginary part of a vectorS\r\n",
    "\r\n",
    "$\\Im \\mathbf{Z}\\rightarrow\\;$ Imaginary part of a matrix\r\n",
    "\r\n",
    "---\r\n",
    "\r\n",
    "$det(\\mathbf{A})\\rightarrow\\;$ Determinant of $\\mathbf{A}$\r\n",
    "\r\n",
    "$Tr(\\mathbf{A})\\rightarrow\\;$ Trace of the matrix $\\mathbf{A}$\r\n",
    "\r\n",
    "$diag(\\mathbf{A})\\rightarrow\\;$ Diagonal matrix of the matrix $\\mathbf{A}$, i.e. $(diag(\\mathbf{A}))_{ij} = \\delta_{ij}\\mathbf{A}_{ij}$\r\n",
    "\r\n",
    "$eig(\\mathbf{A})\\rightarrow\\;$ Eigenvalues of the matrix $\\mathbf{A}$\r\n",
    "\r\n",
    "$vec(\\mathbf{A})\\rightarrow\\;$ The vector-version of the matrix $\\mathbf{A}$\r\n",
    "\r\n",
    "$sup\\rightarrow\\;$ Supremum of a set\r\n",
    "\r\n",
    "$\\Vert\\mathbf{A}\\Vert\\rightarrow\\;$ Matrix norm (subscript if any denotes what norm)\r\n",
    "\r\n",
    "$\\mathbf{A}^{T}\\rightarrow\\;$ Transposed matrix\r\n",
    "\r\n",
    "$\\mathbf{A}^{-T}\\rightarrow\\;$ The inverse of the transposed and vice versa, $\\mathbf{A}^{-T} = (\\mathbf{A}^{-1})^{T} = (\\mathbf{A}^{T})^{-1}$\r\n",
    "\r\n",
    "$\\mathbf{A}^{\\star}\\rightarrow\\;$ Complex conjugated matrix\r\n",
    "\r\n",
    "$\\mathbf{A}^{H}\\rightarrow\\;$ Transposed and complex conjugated matrix (Hermitian)\r\n",
    "\r\n",
    "---\r\n",
    "\r\n",
    "$\\mathbf{A}\\circ\\mathbf{B}$ Hadamard (elementwise) product\r\n",
    "\r\n",
    "$\\mathbf{A}\\otimes\\mathbf{B}$ Kronecker product\r\n",
    "\r\n",
    "---\r\n",
    "\r\n",
    "$\\mathbf{0}\\rightarrow\\;$ The null matrix. Zero in all entries.\r\n",
    "\r\n",
    "$\\mathbf{I}\\rightarrow\\;$ The idnentity matrix\r\n",
    "\r\n",
    "$\\mathbf{J}^{ij}\\rightarrow\\;$ The single entry matrix, 1 at (i,j) and zero elsewhere\r\n",
    "\r\n",
    "$\\mathbf{\\Sigma}\\rightarrow\\;$ A posisitive definite matrix\r\n",
    "\r\n",
    "$\\mathbf{\\Lambda}\\rightarrow\\;$ A diagonal matrix"
   ],
   "metadata": {}
  },
  {
   "cell_type": "markdown",
   "source": [
    "## 1 Basics\r\n",
    "$$\\begin{align} (\\mathbf{A}\\mathbf{B})^{-1} &= \\mathbf{B}^{-1}\\mathbf{A}^{-1} \\\\ (\\mathbf{ABC\\ldots})^{-1} &= \\ldots\\mathbf{C}^{-1}\\mathbf{B}^{-1}\\mathbf{A}^{-1} \\\\ (\\mathbf{A}^{T})^{-1} &= (\\mathbf{A}^{-1})^{T} \\\\ (\\mathbf{A} + \\mathbf{B})^{T} &= \\mathbf{A}^{T} + \\mathbf{B}^{T} \\\\ (\\mathbf{AB})^{T} &= \\mathbf{B}^{T}\\mathbf{A}^{T} \\\\ (\\mathbf{ABC\\ldots})^{T} &= \\ldots\\mathbf{C}^{T}\\mathbf{B}^{T}\\mathbf{A}^{T} \\\\ (\\mathbf{A}^{H})^{-1} &= (\\mathbf{A}^{-1})^{H} \\\\ (\\mathbf{A} + \\mathbf{B})^{H} &= \\mathbf{B}^{H} + \\mathbf{A}^{H} \\\\ (\\mathbf{AB})^{H} &= \\mathbf{B}^{H}\\mathbf{A}^{H} \\\\ (\\mathbf{ABC\\ldots})^{H} &= \\ldots\\mathbf{C}^{H}\\mathbf{B}^{H}\\mathbf{A}^{H} \\\\ \\end{align}$$"
   ],
   "metadata": {}
  },
  {
   "cell_type": "markdown",
   "source": [
    "### 1 Basics Proofs\r\n",
    "- equation (1)):$(\\mathbf{A}\\mathbf{B})^{-1} = \\mathbf{B}^{-1}\\mathbf{A}^{-1}$\r\n",
    "Multiply both side with $AB \\Rightarrow (\\mathbf{A}\\mathbf{B})^{-1}\\mathbf{AB} = \\mathbf{B}^{-1}\\mathbf{A}^{-1}\\mathbf{AB}$\r\n",
    "Now, $LHS = (\\mathbf{A}\\mathbf{B})^{-1}\\mathbf{AB}=\\mathbf{I} \\text{ and } RHS = \\mathbf{B}^{-1}\\mathbf{A}^{-1}\\mathbf{AB}=\\mathbf{B}^{-1}\\mathbf{I}\\mathbf{B} =\\mathbf{I} = LHS$\r\n",
    "\r\n",
    "---\r\n",
    "\r\n",
    "- equation (2):$(\\mathbf{ABC\\ldots})^{-1} = \\ldots\\mathbf{C}^{-1}\\mathbf{B}^{-1}\\mathbf{A}^{-1}$\r\n",
    "This is generalized case of equation (1) and can be proved similarly.\r\n",
    "> generalized 广义\r\n",
    "\r\n",
    "---\r\n",
    "\r\n",
    "- equation (3):$(\\mathbf{A}^{T})^{-1} = (\\mathbf{A}^{-1})^{T}$\r\n",
    "$$\\begin{aligned} RHS &= (\\mathbf{A}^{-1})^{T} \\\\&= (\\mathbf{A}^{-1})^{T}\\mathbf{A}^T(\\mathbf{A}^T)^{-1} \\quad \\because \\mathbf{A}^T(\\mathbf{A}^T)^{-1}=\\mathbf{I} \\\\&=(\\mathbf{AA^{-1}})^T(\\mathbf{A^T})^{-1} \\quad \\because \\mathbf{B^T}\\mathbf{A^T}=(\\mathbf{AB})^T \\quad \\text{See proof of equation (5) for this} \\\\&=\\mathbf{I^T(A^T)^{-1}}\\\\&=\\mathbf{(A^T)^{-1}}\\\\&=LHS\\end{aligned}$$\r\n",
    "\r\n",
    "---\r\n",
    "\r\n",
    "- equation (4):$(\\mathbf{A} + \\mathbf{B})^{T} = \\mathbf{A}^{T} + \\mathbf{B}^{T}$\r\n",
    "The $(i,j)^{th}$ element of $(\\mathbf A^T+\\mathbf B^T)$ is the sum of $(i,j)^{th}$ elements of $\\mathbf A^T$ and $\\mathbf B^T$, which are $(j,i)^{th}$ element of $\\mathbf A$ and $\\mathbf B$, respectively. Thus the $(i,j)^{th}$ element of $\\mathbf A^T+\\mathbf B^T$ is the $(j,i)^{th}$ element of the sum of $\\mathbf A$ and $\\mathbf B$, which is equal to the $(i,j)^{th}$ element of the transpose $(\\mathbf {A+B})^T$.\r\n",
    "\r\n",
    "---\r\n",
    "\r\n",
    "- equation (5):$(\\mathbf{AB})^{T} = \\mathbf{B}^{T}\\mathbf{A}^{T}$\r\n",
    "$$(ab)^T_{ki} = (ab)_{ik} = \\sum_{j=1}^na_{ij}b_{jk}$$\r\n",
    "$$(a^Tb^T)_{ki} = \\sum_{j=1}^nb^T_{kj}a^T_{ji} = \\sum_{j=1}^nb_{jk}a_{ij} =\\sum_{j=1}^na_{ij}b_{jk} = (ab)^T_{ki}$$\r\n",
    "\r\n",
    "---\r\n",
    "\r\n",
    "- equation (6):$(\\mathbf{ABC\\ldots})^{T} = \\ldots\\mathbf{C}^{T}\\mathbf{B}^{T}\\mathbf{A}^{T}$\r\n",
    "This is generalized form of above equation (5). To extend it to more than two matrices, use induction:\r\n",
    "Suppose that for some $n$, we have\r\n",
    "$$\\begin{aligned}\\mathbf{(A_1A_2\\cdots A_n)^T} = \\mathbf{A^T_n \\cdots A^T_2A^T_1} \\tag{proof 1-6-1}\\end{aligned}$$\r\n",
    "Note that we have already derived (5) for $n=2$.\r\n",
    "Then, using the two matrix result and (proof 1-6-1), we have\r\n",
    "$$\\begin{aligned}\\mathbf{(A_1A_2\\cdots A_nA_{n+1})^T} &= \\mathbf{((A_1A_2\\cdots A_n)A_{n+1})^T}\\\\&=\\mathbf{A_{n+1}^T(A_1A_2\\cdots A_n)^T}\\\\&=\\mathbf{A_{n+1}^TA_{n}^T\\cdots A_{2}^TA_{1}^T}\\end{aligned}$$\r\n",
    "\r\n",
    "---\r\n",
    "\r\n",
    "- equation (7):$(\\mathbf{A}^{H})^{-1} = (\\mathbf{A}^{-1})^{H}$\r\n",
    "$$\\begin{aligned}RHS &= \\mathbf{(A^{-1})^H} \\\\&= \\mathbf{(A^{-1})^H A^H (A^H)^{-1}} \\\\&= \\mathbf{(AA^{-1})^H (A^T)^{-1}} \\quad \\because \\mathbf{B^H A^H = (AB)^H} \\text{ See proof of equation (9) fro this} \\\\&= \\mathbf{I^H (A^H)^{-1}} \\\\&= \\mathbf{(A^H)^{-1}} \\\\&= LHS\\end{aligned}$$\r\n",
    "---\r\n",
    "\r\n",
    "- equation (8):$(\\mathbf{A} + \\mathbf{B})^{H} = \\mathbf{B}^{H} + \\mathbf{A}^{H}$\r\n",
    "\r\n",
    "---\r\n",
    "\r\n",
    "- equation (9):$(\\mathbf{AB})^{H} = \\mathbf{B}^{H}\\mathbf{A}^{H}$\r\n",
    "\r\n",
    "---\r\n",
    "\r\n",
    "- equation (10):$(\\mathbf{ABC\\ldots})^{H} = \\ldots\\mathbf{C}^{H}\\mathbf{B}^{H}\\mathbf{A}^{H}$\r\n"
   ],
   "metadata": {}
  },
  {
   "cell_type": "markdown",
   "source": [
    "> Left Hand Side (LHS) 左手边;Right Hand Side (RHS) 右手边"
   ],
   "metadata": {}
  },
  {
   "cell_type": "markdown",
   "source": [
    "### 1 Basics Validate"
   ],
   "metadata": {}
  },
  {
   "cell_type": "code",
   "execution_count": 2,
   "source": [
    "# lets play with the above equations and equatities to see for ouselves\r\n",
    "# caution the above probably work only for square matrices\r\n",
    "width = 3\r\n",
    "height = 3\r\n",
    "A = np.random.random([width, height])\r\n",
    "B = np.random.random([width, height])\r\n",
    "C = np.random.random([width, height])\r\n",
    "\r\n",
    "a = np.random.random([width, 1])\r\n",
    "\r\n",
    "def validate(left, right, eqn):\r\n",
    "    print(\"方程({})的结果: {}\".format(eqn, left.all() == right.all()))\r\n",
    "\r\n",
    "# equation 1:\r\n",
    "lft_hand = np.linalg.inv(A.dot(B))\r\n",
    "rgt_hand = np.dot(np.linalg.inv(B), np.linalg.inv(A))\r\n",
    "validate(lft_hand, rgt_hand, 1)\r\n",
    "\r\n",
    "# equation 2:\r\n",
    "lft_hand = np.linalg.inv(A.dot(B).dot(C))\r\n",
    "rgt_hand = np.dot(np.linalg.inv(C), np.linalg.inv(B)).dot(np.linalg.inv(A))\r\n",
    "validate(lft_hand, rgt_hand, 2)\r\n",
    "\r\n",
    "# equation 3:\r\n",
    "lft_hand = np.linalg.inv(A.T)\r\n",
    "rgt_hand = np.transpose(np.linalg.inv(A))\r\n",
    "validate(lft_hand, rgt_hand, 3)\r\n",
    "\r\n",
    "# equation 4:\r\n",
    "lft_hand = (A+B).T\r\n",
    "rgt_hand = A.T+B.T\r\n",
    "validate(lft_hand, rgt_hand, 4)\r\n",
    "\r\n",
    "# equation 5:\r\n",
    "lft_hand = A.dot(B).T\r\n",
    "rgt_hand = B.T.dot(A.T)\r\n",
    "validate(lft_hand, rgt_hand, 5)\r\n",
    "\r\n",
    "# equation 7:\r\n",
    "lft_hand = np.linalg.inv(np.conjugate(A))\r\n",
    "rgt_hand = np.conjugate(np.linalg.inv(A))\r\n",
    "validate(lft_hand, rgt_hand, 7)\r\n",
    "\r\n",
    "# equation 7:\r\n",
    "lft_hand = np.linalg.inv(np.conjugate(A))\r\n",
    "rgt_hand = np.conjugate(np.linalg.inv(A))\r\n",
    "validate(lft_hand, rgt_hand, 7)\r\n",
    "\r\n",
    "# equation 8:\r\n",
    "lft_hand = np.conjugate(A+B)\r\n",
    "rgt_hand = np.conjugate(A) + np.conjugate(B)\r\n",
    "validate(lft_hand, rgt_hand, 8)\r\n",
    "\r\n",
    "# equation 9:\r\n",
    "lft_hand = np.conjugate(A.dot(B))\r\n",
    "rgt_hand = np.conjugate(B).dot(np.conjugate(A))\r\n",
    "validate(lft_hand, rgt_hand, 9)"
   ],
   "outputs": [
    {
     "output_type": "stream",
     "name": "stdout",
     "text": [
      "方程(1)的结果: True\n",
      "方程(2)的结果: True\n",
      "方程(3)的结果: True\n",
      "方程(4)的结果: True\n",
      "方程(5)的结果: True\n",
      "方程(7)的结果: True\n",
      "方程(7)的结果: True\n",
      "方程(8)的结果: True\n",
      "方程(9)的结果: True\n"
     ]
    }
   ],
   "metadata": {}
  },
  {
   "cell_type": "markdown",
   "source": [
    "### 1.1 Trace\r\n",
    "$$\\begin{align} Tr(\\mathbf{A}) &= \\sum_{i} \\mathbf{A}_{ii} \\\\ Tr(\\mathbf{A}) &= \\sum_{i}\\lambda_{i}, \\;\\;\\lambda_{i} = eig(\\mathbf{A}) \\\\ Tr(\\mathbf{A}) &= Tr(\\mathbf{A}^{T}) \\\\ Tr(\\mathbf{AB}) &= Tr(\\mathbf{BA}) \\\\ Tr(\\mathbf{A}+\\mathbf{B}) &= Tr(\\mathbf{A}) + Tr(\\mathbf{B}) \\\\ Tr(\\mathbf{ABC}) &= Tr(\\mathbf{BCA}) = Tr(\\mathbf{CAB}) \\\\ \\vec{a}^{T}\\vec{a} &= Tr(\\vec{a}\\vec{a}^{T}) \\end{align}$$"
   ],
   "metadata": {}
  },
  {
   "cell_type": "markdown",
   "source": [
    "#### 1.1 Trace Proofs\r\n",
    "\r\n",
    "- equation (11):$Tr(\\mathbf{A}) = \\sum_{i} \\mathbf{A}_{ii}$\r\n",
    "By definition of trace of the matrix, which is the sum of elements on the main diagonal of $\\mathbf{A}$.\r\n",
    "\r\n",
    "---\r\n",
    "\r\n",
    "- equation (12):$Tr(\\mathbf{A}) = \\sum_{i}\\lambda_{i}, \\;\\;\\lambda_{i} = eig(\\mathbf{A})$\r\n",
    "By definition, the characteristic polynomial of an $n \\times n$ matrix $\\mathbf{A}$ is given by\r\n",
    "$$p(t) = \\operatorname{det}(\\mathbf{A-tI}) = (-1)^n \\Big( t^n - (\\operatorname{tr}\\mathbf A)t^{n-1} + \\cdots + (-1)^n \\operatorname{det}\\mathbf{A} \\Big)$$\r\n",
    "On the other hand, $p(t)=(−1)^n(t−\\lambda_1)\\cdots(t−\\lambda_n)$, where the $\\lambda_j$ are the eigenvalues of $\\mathbf A$. So, comparing coefficients, we have $\\operatorname{tr}\\mathbf A=\\lambda_1+\\cdots+\\lambda_n$.\r\n",
    "\r\n",
    "---\r\n",
    "\r\n",
    "- equation (13):$Tr(\\mathbf{A}) = Tr(\\mathbf{A}^{T})$\r\n",
    "Elements of any matrix $\\mathbf{A}$ can be represented by $\\mathbf{A}_{ij}$. After transpose, the corresponding becomes $\\mathbf{A}_{ji}$. But for diagonal elements, $i=j$, therefore, from definition of trace of matrix $\\operatorname{Tr}(\\mathbf A)=\\operatorname{Tr}(\\mathbf A^T)= \\sum_i \\mathbf A_{ii}$\r\n",
    "\r\n",
    "---\r\n",
    "\r\n",
    "- equation (14):$Tr(\\mathbf{AB}) = Tr(\\mathbf{BA})$\r\n",
    "Let $\\mathbf{A}$ be a $n \\times m$ and \\mathbf{B} be a $m \\times n$ matrix, we have\r\n",
    "$$\\begin{aligned}\\operatorname{Tr}(\\mathbf {AB}) &= \\sum_{i=1}^n(\\mathbf{AB})_{ii} \\\\&=\\sum_{i=1}^n\\sum_{j=1}^m \\mathbf {A}_{ij} \\mathbf {B}_{ji} \\\\&= \\sum_{j=1}^m\\sum_{i=1}^n \\mathbf {B}_{ji} \\mathbf {A}_{ij} \\\\&= \\sum_{j=1}^m(\\mathbf{BA})_{jj} \\\\&= \\operatorname{Tr}(\\mathbf{BA})\\end{aligned}$$\r\n",
    "\r\n",
    "---\r\n",
    "\r\n",
    "- equation (15):$Tr(\\mathbf{A}+\\mathbf{B}) = Tr(\\mathbf{A}) + Tr(\\mathbf{B})$\r\n",
    "$$\\begin{aligned}RHS &= \\operatorname{Tr}(\\mathbf A) + \\operatorname{Tr}(\\mathbf B) \\\\&=\\sum_{k=1}^na_{kk} + \\sum_{k=1}^nb_{kk} \\\\&=\\sum_{k=1}^n(a_{kk} + b_{kk}) \\\\&= \\operatorname{Tr}(\\mathbf{A}+\\mathbf{B}) \\\\&=LHS \\end{aligned}$$\r\n",
    "\r\n",
    "---\r\n",
    "\r\n",
    "- equation (16):$Tr(\\mathbf{ABC}) = Tr(\\mathbf{BCA}) = Tr(\\mathbf{CAB})$\r\n",
    "More general form of (proof 14).\r\n",
    "\r\n",
    "---\r\n",
    "\r\n",
    "- equation (17):$\\mathbf{a^Ta} = Tr(\\mathbf{aa^T})$"
   ],
   "metadata": {}
  },
  {
   "cell_type": "markdown",
   "source": [
    "#### 1.1 Trace Validate"
   ],
   "metadata": {}
  },
  {
   "cell_type": "code",
   "execution_count": 3,
   "source": [
    "# equation 11:\r\n",
    "lft_hand = np.trace(A)\r\n",
    "rgt_hand = np.sum(np.diag(A))\r\n",
    "validate(lft_hand, rgt_hand, 11)\r\n",
    "\r\n",
    "# equation 12:\r\n",
    "lft_hand = np.trace(A)\r\n",
    "rgt_hand = np.sum(np.linalg.eigvals(A))\r\n",
    "validate(lft_hand, rgt_hand, 12)\r\n",
    "\r\n",
    "# equation 13:\r\n",
    "lft_hand = np.trace(A)\r\n",
    "rgt_hand = np.trace(A.T)\r\n",
    "validate(lft_hand, rgt_hand, 13)\r\n",
    "\r\n",
    "# equation 14:\r\n",
    "lft_hand = np.trace(A.dot(B))\r\n",
    "rgt_hand = np.trace(B.dot(A))\r\n",
    "validate(lft_hand, rgt_hand, 14)\r\n",
    "\r\n",
    "# equation 15:\r\n",
    "lft_hand = np.trace(A+B)\r\n",
    "rgt_hand = np.trace(A) + np.trace(B)\r\n",
    "validate(lft_hand, rgt_hand, 15)\r\n",
    "\r\n",
    "# equation 16:\r\n",
    "lft_hand = np.trace(np.dot(A.dot(B), C))\r\n",
    "rgt_hand = np.trace(np.dot(B.dot(C), A))\r\n",
    "validate(lft_hand, rgt_hand, 16)\r\n",
    "\r\n",
    "# equation 17:\r\n",
    "lft_hand = np.dot(a.T, a)\r\n",
    "rgt_hand = np.trace(np.dot(a, a.T))\r\n",
    "validate(lft_hand, rgt_hand, 17)"
   ],
   "outputs": [
    {
     "output_type": "stream",
     "name": "stdout",
     "text": [
      "方程(11)的结果: True\n",
      "方程(12)的结果: True\n",
      "方程(13)的结果: True\n",
      "方程(14)的结果: True\n",
      "方程(15)的结果: True\n",
      "方程(16)的结果: True\n",
      "方程(17)的结果: True\n"
     ]
    }
   ],
   "metadata": {}
  },
  {
   "cell_type": "markdown",
   "source": [
    "### 1.2 Determinant\r\n",
    "Let $A$ be an $n \\times n$ matrix.\r\n",
    "$$\\begin{align} \\operatorname{det}(\\mathbf{A}) &= \\prod_i{\\lambda_i} \\quad \\lambda_i=\\operatorname{eig}(\\mathbf{A})\\\\ \\operatorname{det}(c\\mathbf{A}) &=c^n \\operatorname{det}(\\mathbf{A}), \\quad \\text{if } \\mathbf{A} \\in \\mathbb{R}^{n \\times n} \\\\ \\operatorname{det}(\\mathbf{A}^T) &=\\operatorname{det}(\\mathbf{A}) \\\\ \\operatorname{det}(\\mathbf{AB}) &=\\operatorname{det}(\\mathbf{A})\\operatorname{det}(\\mathbf{B}) \\\\ \\operatorname{det}(\\mathbf{A}^{-1}) &= 1/\\operatorname{det}(\\mathbf{A}) \\\\ \\operatorname{det}(\\mathbf{A}^{n}) &= \\operatorname{det}(\\mathbf{A})^n \\\\ \\operatorname{det}(\\mathbf{I+uv^T}) &= 1+\\mathbf{u^Tv} \\\\ \\end{align}$$\r\n",
    "\r\n",
    "For $n=2$:\r\n",
    "\r\n",
    "$$\\begin{align} \\operatorname{det}(\\mathbf{I+A}) = 1+\\operatorname{det}(\\mathbf{A})+\\operatorname{Tr}(\\mathbf{A}) \\end{align}$$\r\n",
    "\r\n",
    "For $n=3$:\r\n",
    "\r\n",
    "$$\\begin{align} \\operatorname{det}(\\mathbf{I+A}) = 1+\\operatorname{det}(\\mathbf{A})+\\operatorname{Tr}(\\mathbf{A})+\\frac{1}{2}\\operatorname{Tr}(\\mathbf{A})^2-\\frac{1}{2}\\operatorname{Tr}(\\mathbf{A}^2) \\end{align}$$\r\n",
    "\r\n",
    "For $n=4$:\r\n",
    "\r\n",
    "$$\\begin{equation}\\begin{aligned} \\operatorname{det}(\\mathbf{I+A}) =\\; &1+\\operatorname{det}(\\mathbf{A})+\\operatorname{Tr}(\\mathbf{A})\\\\ &+\\frac{1}{2}\\operatorname{Tr}(\\mathbf{A})^2-\\frac{1}{2}\\operatorname{Tr}(\\mathbf{A}^2)\\\\ &+\\frac{1}{6}\\operatorname{Tr}(\\mathbf{A})^3-\\frac{1}{2}\\operatorname{Tr}(\\mathbf{A})\\operatorname{Tr}(\\mathbf{A}^2)+\\frac{1}{3}\\operatorname{Tr}(\\mathbf{A}^3) \\\\ \\end{aligned}\\end{equation}$$\r\n",
    "\r\n",
    "For small $\\varepsilon$, the following approximation holds\r\n",
    "对于小$\\varepsilon$，以下近似成立\r\n",
    "\r\n",
    "$$\\begin{align} \\operatorname{det}(\\mathbf{I+\\varepsilon A}) \\cong 1+\\operatorname{det}(\\mathbf{A})+\\varepsilon\\operatorname{Tr}(\\mathbf{A})+\\frac{1}{2}\\varepsilon^2\\operatorname{Tr}(\\mathbf{A})^2-\\frac{1}{2}\\varepsilon^2\\operatorname{Tr}(\\mathbf{A}^2) \\end{align}$$\r\n"
   ],
   "metadata": {}
  },
  {
   "cell_type": "markdown",
   "source": [
    "#### 1.2 Determinant Validate"
   ],
   "metadata": {}
  },
  {
   "cell_type": "code",
   "execution_count": 6,
   "source": [
    "# equation 18:\r\n",
    "lft_hand = np.linalg.det(A)\r\n",
    "rgt_hand = np.prod(np.linalg.eigvals(A))\r\n",
    "validate(lft_hand, rgt_hand, 18)"
   ],
   "outputs": [
    {
     "output_type": "stream",
     "name": "stdout",
     "text": [
      "方程(18)的结果: True\n",
      "方程(19)的结果: True\n"
     ]
    }
   ],
   "metadata": {}
  },
  {
   "cell_type": "markdown",
   "source": [
    "### 1.3 The Special Case 2x2 (特殊情况)\r\n"
   ],
   "metadata": {}
  }
 ]
}